

%%%%%%%%%%%%%%%%%%%%%%%%%%%
\documentstyle[11pt]{article}
\hyphenation{U-ni-ver-si-ta com-pu-ta-zio-na-li va-lo-ri u-san-do}
\def\N{\hbox{I\kern-.2em\hbox{N}}}
\def\P{\hbox{I\kern-.2em\hbox{P}}}
\def\R{\hbox{\rm I\kern-.2em\hbox{\rm R}}}
\def\Z{\hbox{\rm Z\kern-4.0pt{\rm Z}}}

\begin{document}
{\bf r\_ia\_1}
$$ x_0=0, \; x_1=1, \; x_2=2 \quad f_0=-1, \; f_1=0, \; f_2=2 $$



$$-(x^2-3x+2)/2+2(x^2-x)/2=0.5x^2+0.5x-1$$


{\bf ria2}
$$ x_0=0, \; x_1=1, \; x_2=2, \; x_3=3 \quad f_0=-1, \; f_1=0, \; f_2=1 \; f_3=0 $$


$$-1+x-1/3 x(x-1)(x-2)$$



{\bf ria3}
$$ x_0=-2, \; x_1=-1, \; x_2=1, \; x_3=2 \quad f_0=0, \; f_1=1, \; f_2=0 \; f_3=1 $$

$$P2(x)=1/10 x+1/2$$

$$ E=0.94868$$


{\bf ria4}

$$ x_0=0, \; x_1=1, \; x_2=2 \quad f_0=-1, \; f_1=0, \; f_2=1 $$


$$s(x)=-1+x+(x-1)_+$$



{\bf ria5}

$$ x_0=0, \; x_1=1, \; x_2=2, \; x_3=3 \quad f_0=-1, \; f_1=0, \; f_2=1 \; f_3=0 $$

$$s(x)=-2+11/3x-14/3(x-1)_+= -2+3.667x-4.667(x-1)_+$$


{\bf ria6}

$$ x_0=0, \; x_1=1, \; x_2=2 \quad f_0=-1, \; f_1=0, \; f_2=1 $$

$$P(x)=-1+x$$
Aggiungere la coppia$(\overline{x},\overline{f})=(1/2,0)$

$$ P(x)=-1+x-4/3x(x-1)(x-2)=-4/3x^3+4x^2-5/3x-1$$

{\bf ria7}
$$ x_0=-2, \; x_1=-1, \; x_2=1, \; x_3=2 \quad f_0=0, \; f_1=1, \; f_2=0 \; f_3=1 $$

$$P2(x)=1/10 x+1/2$$
{\bf ria8}

$$ x_0=0, \; x_1=1, \; x_2=2 \quad f_0=-1, \; f_1=0, \; f_2=1 $$

$$P(x)=-1+x$$

\end{document}
